LeanCats/LitmusParser.lean
@@ -1,13 +1,13 @@
+import LeanCats.Data
 import LeanCats.AST
-import LeanCats.HerdingCats
 
 namespace LitmusParser
 
 def ins2event
   (t_id : Nat)
-  (thread : Primitives.Thread)
+  (thread : Thread)
   (ins : LitmusAST.Instruction)
-  (id : String) : Primitives.Event :=
+  (id : String) : Event :=
   {
     id := id
     t_id := t_id
@@ -16,11 +16,11 @@ def ins2event
     a := ins.action
   }
 
-def prog2events (prog : LitmusAST.Program) (start_id : Nat) : List Primitives.Event × Nat :=
-  let thread : Primitives.Thread := Primitives.Thread.mk prog.thread
+def prog2events (prog : LitmusAST.Program) (start_id : Nat) : List Event × Nat :=
+  let thread : Thread := Thread.mk prog.thread
   let ins2event := ins2event prog.thread thread
 
-  let rec process_instructions (instructions : List LitmusAST.Instruction) (curr_id : Nat) : List Primitives.Event × Nat :=
+  let rec process_instructions (instructions : List LitmusAST.Instruction) (curr_id : Nat) : List Event × Nat :=
     match instructions with
     | [] => ([], curr_id)
     | ins :: rest =>
@@ -31,7 +31,7 @@ def prog2events (prog : LitmusAST.Program) (start_id : Nat) : List Primitives.Ev
 
   process_instructions prog.instructions start_id
 
-def zip_instructions (insts : List Primitives.Event) : Set (Primitives.Event × Primitives.Event) :=
+def zip_instructions (insts : List Event) : Set (Event × Event) :=
   -- [r₁ r₂ r₂] -> [r₁ r₂] [r₂ r₃] -> [(r₁, r₂), (r₂, r₃)]
   -- edge caes: return []
   let insts₁ := insts.eraseIdx 0
@@ -40,29 +40,31 @@ def zip_instructions (insts : List Primitives.Event) : Set (Primitives.Event × 
   let insts := insts₁.zip insts₂
 
   -- accumulate all the relations.
-  insts.foldl Primitives.R.add Primitives.R.empty
-
-def get_po (litmus : LitmusAST.Litmus) : Primitives.Relation :=
-  let start : Nat := 0
-
-  let rec process_programs (program : List LitmusAST.Program) (curr_id : Nat) : List (List Primitives.Event) × Nat :=
-    match program with
-    | [] => ([], curr_id)
-    | prog :: rest =>
-      let (prog_events, next_id) := prog2events prog curr_id
-      let (rest_programs_events, final_id) := process_programs rest next_id
-      (prog_events :: rest_programs_events, final_id)
-
-  let (all_program_events, _) := process_programs litmus.programs start
-
-  let events_list := all_program_events.map zip_instructions
-
-  events_list.foldl Set.union Primitives.R.empty
-
-def get_rf (litmus : LitmusAST.Litmus) : Primitives.Relation :=
+  -- insts.foldl Primitives.R.add Primitives.R.empty
   sorry
 
-def get_fr (litmus : LitmusAST.Litmus) : Primitives.Relation :=
+-- def get_po (litmus : LitmusAST.Litmus) : Relation :=
+--   let start : Nat := 0
+--
+--   let rec process_programs (program : List LitmusAST.Program) (curr_id : Nat) : List (List Event) × Nat :=
+--     match program with
+--     | [] => ([], curr_id)
+--     | prog :: rest =>
+--       let (prog_events, next_id) := prog2events prog curr_id
+--       let (rest_programs_events, final_id) := process_programs rest next_id
+--       (prog_events :: rest_programs_events, final_id)
+--
+--   let (all_program_events, _) := process_programs litmus.programs start
+--
+--   let events_list := all_program_events.map zip_instructions
+--
+--   -- events_list.foldl Set.union R.empty
+--   sorry
+
+def get_rf (litmus : LitmusAST.Litmus) : Relation :=
+  sorry
+
+def get_fr (litmus : LitmusAST.Litmus) : Relation :=
   sorry
 
 -- There are lots of algorithms to find the read-from relation, like use-def chains (worklist to find)
